Fix the names of the typing props. (They haven't been about scoping in a long time now)
part 1: the type names

seplog/typing.v
@@ -18,114 +18,112 @@ Require Import varmap.
 (*
  * well-formedness constraints
  *
- * we have the following constraints:
- *   1. scoping: variables must be used only in their scope.
+ * we have the following major constraints:
+ *   1. scoping: variables must be used only in their scope and not
+ *      redefined when in scope.
  *   2. uniqueness: (local) variable identifiers must be unique across
- *      each entire proc.
+ *      each entire proc. Nowadays this is an immediate consequence of #1.
  *   3. flow: variables must be declared before used.
  *   4. typing: each local variable has exactly one type.
  *
- * "VarsScoped" covers #1 and #3.
- * "VarsUnique" covers #2; it's separate because its environment is
- *     different.
- * "VarsTyped" covers #4.
+ * These are all now covered by the *Typed props.
  *
- * A proc is well-formed if it satisfies all these properties.
- *
- * this is (for now) chiefly about insisting that every variable is declared
- * exactly once. types are mostly enforced by the embedding. we ignore scopes
- * when checking for duplicate declarations, at least for now.
+ * We have the additional constraint that the body of a proc must
+ * end in a return so that the proc can't fall of the end without
+ * providing a return value. (In principle the end could also be
+ * unreachable, or the proc could always diverge, but we don't try
+ * to reason about those cases.)
  *)
 
 (*
  * scoping
  *)
 
-Inductive VarsScopedExpr: forall (t: type), VarMap type -> expr -> Prop :=
+Inductive ExprTyped: forall (t: type), VarMap type -> expr -> Prop :=
 | vars_scoped_value: forall (t: type) env k,
      type_of_value k = t ->
-     VarsScopedExpr t env (e_value t k)
+     ExprTyped t env (e_value t k)
 | vars_scoped_read: forall (t: type) env id,
      VarMapMapsTo (mkvar t id) t env ->
-     VarsScopedExpr t env (e_read (mkvar t id))
+     ExprTyped t env (e_read (mkvar t id))
 | vars_scoped_cond: forall t env pred te fe,
-     VarsScopedExpr t_bool env pred ->
-     VarsScopedExpr t env te ->
-     VarsScopedExpr t env fe ->
-     VarsScopedExpr t env (e_cond t pred te fe)
+     ExprTyped t_bool env pred ->
+     ExprTyped t env te ->
+     ExprTyped t env fe ->
+     ExprTyped t env (e_cond t pred te fe)
 .
 
-Inductive VarsScopedStmt: VarMap type -> stmt -> Prop :=
+Inductive StmtTyped: VarMap type -> stmt -> Prop :=
 | vars_scoped_skip: forall env,
-     VarsScopedStmt env s_skip
+     StmtTyped env s_skip
 | vars_scoped_seq: forall env s1 s2,
-     VarsScopedStmt env s1 ->
-     VarsScopedStmt env s2 ->
-     VarsScopedStmt env (s_seq s1 s2)
+     StmtTyped env s1 ->
+     StmtTyped env s2 ->
+     StmtTyped env (s_seq s1 s2)
 | vars_scoped_start: forall env pt p e,
-     VarsScopedProc pt t_unit p ->
-     VarsScopedExpr pt env e ->
-     VarsScopedStmt env (s_start p e)
+     ProcTyped pt t_unit p ->
+     ExprTyped pt env e ->
+     StmtTyped env (s_start p e)
 | vars_scoped_assign: forall t env id e,
-     VarsScopedExpr t env e ->
+     ExprTyped t env e ->
      VarMapMapsTo (mkvar t id) t env ->
-     VarsScopedStmt env (s_assign (mkvar t id) e)
+     StmtTyped env (s_assign (mkvar t id) e)
 | vars_scoped_load: forall t env id e,
-     VarsScopedExpr (t_addr t) env e ->
+     ExprTyped (t_addr t) env e ->
      VarMapMapsTo (mkvar t id) t env ->
-     VarsScopedStmt env (s_load (mkvar t id) e)
+     StmtTyped env (s_load (mkvar t id) e)
 | vars_scoped_store: forall t env lid e,
      VarMapMapsTo (mkvar (t_addr t) lid) (t_addr t) env ->
-     VarsScopedExpr t env e ->
-     VarsScopedStmt env (s_store (mkvar (t_addr t) lid) e)
+     ExprTyped t env e ->
+     StmtTyped env (s_store (mkvar (t_addr t) lid) e)
 | vars_scoped_if: forall env pred ts fs,
-     VarsScopedExpr t_bool env pred ->
-     VarsScopedStmt env ts ->
-     VarsScopedStmt env fs ->
-     VarsScopedStmt env (s_if pred ts fs)
+     ExprTyped t_bool env pred ->
+     StmtTyped env ts ->
+     StmtTyped env fs ->
+     StmtTyped env (s_if pred ts fs)
 | vars_scoped_while: forall env pred body,
-     VarsScopedExpr t_bool env pred ->
-     VarsScopedStmt env body ->
-     VarsScopedStmt env (s_while pred body)
+     ExprTyped t_bool env pred ->
+     StmtTyped env body ->
+     StmtTyped env (s_while pred body)
 | vars_scoped_call: forall env pt rt id p arg,
-     VarsScopedProc pt rt p ->
-     VarsScopedExpr pt env arg ->
+     ProcTyped pt rt p ->
+     ExprTyped pt env arg ->
      VarMapMapsTo (mkvar rt id) rt env ->
-     VarsScopedStmt env (s_call (mkvar rt id) p arg)
+     StmtTyped env (s_call (mkvar rt id) p arg)
 | vars_scoped_return: forall t env e,
      (* XXX this doesn't check against the proc type... *)
-     VarsScopedExpr t env e ->
-     VarsScopedStmt env (s_return e)
+     ExprTyped t env e ->
+     StmtTyped env (s_return e)
 | vars_scoped_getlock: forall t env id,
-     VarsScopedStmt env (s_getlock (mkvar (t_lock t) id))
+     StmtTyped env (s_getlock (mkvar (t_lock t) id))
 | vars_scoped_putlock: forall t env id,
-     VarsScopedStmt env (s_getlock (mkvar (t_lock t) id))
+     StmtTyped env (s_getlock (mkvar (t_lock t) id))
 with
 
-(*Inductive*) VarsScopedVardecl: VarMap type -> vardecl ->
+(*Inductive*) VardeclTyped: VarMap type -> vardecl ->
                                  VarMap type -> Prop :=
 | vars_scoped_vardecl: forall t env id e,
-     VarsScopedExpr t env e ->
+     ExprTyped t env e ->
      ~(VarMapIn (mkvar t id) env) ->
-     VarsScopedVardecl env (mkvardecl (mkvar t id) e) (VarMap_add (mkvar t id) t env)
+     VardeclTyped env (mkvardecl (mkvar t id) e) (VarMap_add (mkvar t id) t env)
 with
 
-(*Inductive*) VarsScopedVardecls: VarMap type -> list vardecl ->
+(*Inductive*) VardeclsTyped: VarMap type -> list vardecl ->
                                   VarMap type -> Prop :=
 | vars_scoped_vardecls_nil: forall env,
-     VarsScopedVardecls env [] env
+     VardeclsTyped env [] env
 | vars_scoped_vardecls_cons: forall env decl env' decls env'',
-     VarsScopedVardecl env decl env' ->
-     VarsScopedVardecls env' decls env'' ->
-     VarsScopedVardecls env (decl :: decls) env''
+     VardeclTyped env decl env' ->
+     VardeclsTyped env' decls env'' ->
+     VardeclsTyped env (decl :: decls) env''
 with
 
-(*Inductive*) VarsScopedProc: forall pt rt, proc -> Prop :=
+(*Inductive*) ProcTyped: forall pt rt, proc -> Prop :=
 | vars_scoped_proc: forall pt rt id decls body env,
-     VarsScopedVardecls (VarMap_add (mkvar pt id) pt (VarMap_empty type))
+     VardeclsTyped (VarMap_add (mkvar pt id) pt (VarMap_empty type))
                         decls env ->
-     VarsScopedStmt env body ->
-     VarsScopedProc pt rt (mkproc rt (mkvar pt id) decls body)
+     StmtTyped env body ->
+     ProcTyped pt rt (mkproc rt (mkvar pt id) decls body)
 .
 
 
@@ -135,7 +133,7 @@ with
 
 (*
  * This differs in that the environment doesn't nest. Also,
- * it doesn't reason about exprs; it relies on VarsScoped to
+ * it doesn't reason about exprs; it relies on Typed to
  * make sure they refer only to variables that exist.
  *)
 
@@ -218,12 +216,12 @@ with
 
 
 Definition StmtOk s : Prop :=
-   (forall env, VarsScopedStmt env s) /\
+   (forall env, StmtTyped env s) /\
    (forall env, VarsUniqueStmt s env)
 .
 
 Definition ProcOk pt rt (p: proc): Prop :=
-   (VarsScopedProc pt rt p) /\
+   (ProcTyped pt rt p) /\
    (VarsUniqueProc p) /\
    ProcReturnOk rt p
 .
